Restructuring of Show, Assemble and Testing

Uppaal_Networks/AbsInt/AbsInt_Test.thy
@@ -1,96 +1,9 @@
 theory AbsInt_Test
-  imports AbsInt_Refine "HOL-IMP.AExp" "HOL.String"
+  imports
+    "HOL.String"
+    AbsInt_Refine
+    Uppaal_Networks.UPPAAL_Asm_Show
 begin
-
-fun assemble :: "instr list \<Rightarrow> spaced_program" where
-  "assemble listing = SpacedProgram
-    (set (upt 0 (length listing)))
-    (\<lambda>pc. if pc < length listing then Some (listing ! pc) else None)"
-
-class "show" =
-  fixes "show" :: "'a \<Rightarrow> string"
-
-fun hexlit :: "nat \<Rightarrow> nat \<Rightarrow> string" where
-  "hexlit 0 0 = ''0x''" |
-  "hexlit len v =
-    (let c = v mod 16 in
-    hexlit (len-1) (v div 16) @ [char_of (if c < 10 then 48 + c else 97 + (c - 10))])"
-
-fun hexliti :: "nat \<Rightarrow> int \<Rightarrow> string" where
-  "hexliti len v = hexlit len (if v < 0 then nat (-v) else nat v)"
-
-instantiation nat :: "show"
-begin
-fun show_nat :: "nat \<Rightarrow> string" where
-  "show_nat n = hexlit 4 n"
-instance proof qed
-end
-
-instantiation int :: "show"
-begin
-fun show_int :: "int \<Rightarrow> string" where
-  "show_int n = hexliti 1 n"
-instance proof qed
-end
-
-instantiation bool :: "show"
-begin
-fun show_bool :: "bool \<Rightarrow> string" where
-  "show_bool True = ''True''" |
-  "show_bool False = ''False''"
-instance proof qed
-end
-
-instantiation instr :: "show"
-begin
-fun show_instr :: "instr \<Rightarrow> string" where
-  "show_instr (JMPZ a) = ''JMPZ '' @ (show a)" |
-  "show_instr ADD = ''ADD''" |
-  "show_instr NOT = ''NOT''" |
-  "show_instr AND = ''AND''" |
-  "show_instr instr.LT = ''LT''" |
-  "show_instr instr.LE = ''LE''" |
-  "show_instr instr.EQ = ''EQ''" |
-  "show_instr (PUSH imm) = ''PUSH '' @ (show imm)" |
-  "show_instr POP = ''POP''" |
-  "show_instr (LID r) = ''LID '' @ (show r)"|
-  "show_instr STORE = ''STORE''" |
-  "show_instr (STOREI r imm) = ''STOREI '' @ (show r) @ '' '' @ (show imm)"|
-  "show_instr COPY = ''COPY''" |
-  "show_instr CALL = ''CALL''" |
-  "show_instr RETURN = ''RETURN''" |
-  "show_instr HALT = ''HALT''" |
-  "show_instr (STOREC n i) = ''STOREC '' @ (show n) @ '' '' @ (show i)" |
-  "show_instr (SETF b) = ''SETF '' @ (show b)"
-instance ..
-end
-
-instantiation prod :: ("show", "show") "show"
-begin
-fun show_prod :: "('a * 'b) \<Rightarrow> string" where
-  "show_prod (a, b) = CHR ''('' # show a @ '', '' @ show b @ '')''"
-instance ..
-end
-
-instantiation list :: ("show") "show"
-begin
-fun show_list_rest :: "'a list \<Rightarrow> string" where
-  "show_list_rest [] = '']''" |
-  "show_list_rest (x # xs) = show x @ '', '' @ show_list_rest xs"
-
-fun show_list :: "'a list \<Rightarrow> string" where
-  "show_list [] = ''[]''" |
-  "show_list xs = show_list_rest xs"
-instance ..
-end
-
-instantiation option :: ("show") "show"
-begin
-fun show_option :: "'a option \<Rightarrow> string" where
-  "show_option None = ''None''" |
-  "show_option (Some x) = ''Some '' @ show x"
-instance ..
-end
 
 instantiation dumb_base :: "show"
 begin
@@ -99,78 +12,33 @@ fun show_dumb_base :: "dumb_base \<Rightarrow> string" where
 instance ..
 end
 
-abbreviation init where "init \<equiv> (0, [], [], False, [])"
-value "case assemble myprog of (SpacedProgram space prog) \<Rightarrow> step (the (prog (state_pc init))) init"
-
-instantiation spaced_program :: "show"
-begin
-fun show_spaced_program :: "spaced_program \<Rightarrow> string" where
-  "show_spaced_program (SpacedProgram space prog) =
-    concat (map (\<lambda>pc. (show pc) @ '' '' @ (show (the (prog pc))) @ [char_of (10::nat)]) (sorted_list_of_set space))"
-instance proof qed
-end
-
-definition "asm_width \<equiv> 20"
-datatype 'a dispctx = DisplayCtx spaced_program "'a state_map"
-
-definition "emoji \<equiv> map char_of ([240,159,164,183] :: nat list)"
-
-fun intercalate:: "'a list \<Rightarrow> 'a list list \<Rightarrow> 'a list" where
-  "intercalate _ [] = []" |
-  "intercalate _ [x] = x" |
-  "intercalate sep (x # xs) = x @ sep @ intercalate sep xs"
-
-fun format_ctx_line :: "nat \<Rightarrow> addr \<Rightarrow> program \<Rightarrow> 'a::show \<Rightarrow> string" where
-  "format_ctx_line len pc prog v =
-      (let asm = (show pc) @ '' '' @ (case prog pc of Some op \<Rightarrow> show op | None \<Rightarrow> ''--'');
-           padding = replicate ((asm_width - 1) - length asm + 1) CHR '' '';
-           states = show v in
-      asm @ padding @ states @ ''\<newline>'')"
-
-instantiation dispctx :: ("show") "show"
-begin
-fun show_dispctx :: "'a dispctx \<Rightarrow> string" where
-  "show_dispctx (DisplayCtx (SpacedProgram space prog) st) =
-    concat (map (\<lambda>pc. format_ctx_line asm_width pc prog (lookup st pc)) (sorted_list_of_set space))"
-instance proof qed
-end
-
-
-definition myprog :: "instr list" where "myprog \<equiv> [
-CALL,
+definition "myprog_listing \<equiv> [
 PUSH 42,
 PUSH 3,
 instr.LT,
+JMPZ 7,
+HALT,
+PUSH 13,
+PUSH 37,
+PUSH 123,
 HALT
 ]"
 
-definition "mysprog \<equiv> assemble myprog"
-
-fun spprog :: "spaced_program \<Rightarrow> program" where
-  "spprog (SpacedProgram _ prog) = prog"
-
-definition "empty_state \<equiv> ([], [], False, [])"
-definition "empty_state1 \<equiv> ([], [], True, [])"
-
-definition "(collect_result::collect_state set state_map) \<equiv>
-  let prog = spprog mysprog;
-      entry = deepen {(0::addr, empty_state), (0, empty_state1)} in
-  collect_loop prog 4 entry"
+definition "myprog \<equiv> assemble myprog_listing"
 
 definition "dumb_entry \<equiv> merge_single (\<bottom>::dumb state_map) 0 (Some Any)"
 
 definition "dumb_stepped \<equiv>
-  step_map dumb_step (spprog mysprog) dumb_entry"
+  step_map dumb_step (fetch_op myprog) dumb_entry"
 value "lookup (dump_stepped::dumb state_map) 0"
 
 definition "dumb_advanced \<equiv>
-  advance dumb_step (spprog mysprog) dumb_entry"
+  advance dumb_step (fetch_op myprog) dumb_entry"
 
 definition "dumb_result \<equiv>
-  Dumb.ai_loop (spprog mysprog) 1 dumb_entry"
+  Dumb.ai_loop (fetch_op myprog) 100 dumb_entry"
 
-value "dumb_result"
-definition "abs_res_str \<equiv> String.implode (show (DisplayCtx mysprog dumb_result))"
+definition "abs_res_str \<equiv> String.implode (show (DisplayCtx myprog dumb_result))"
 ML \<open>val _ = writeln (@{code abs_res_str})\<close>
 
 (*
@@ -190,7 +58,16 @@ fun show_set :: "'a set \<Rightarrow> string" where
 instance proof qed
 end
 
+definition "empty_state \<equiv> ([], [], False, [])"
+definition "empty_state1 \<equiv> ([], [], True, [])"
+
+definition "(collect_result::collect_state set state_map) \<equiv>
+  let prog = fetch_op myprog;
+      entry = deepen {(0::addr, empty_state), (0, empty_state1)} in
+  collect_loop prog 4 entry"
+
 definition "my_string \<equiv> String.implode (show (DisplayCtx mysprog collect_result))"
-ML \<open>val _ = writeln (@{code my_string})\<close>*)
+ML \<open>val _ = writeln (@{code my_string})\<close>
+*)
 
 end
