Uppaal_Networks/UPPAAL_Asm_Show.thy
@@ -1,0 +1,128 @@
+theory UPPAAL_Asm_Show
+  imports
+    UPPAAL_Asm_Map
+    UPPAAL_Asm_Assemble
+begin
+
+class "show" =
+  fixes "show" :: "'a \<Rightarrow> string"
+
+fun hexlit :: "nat \<Rightarrow> nat \<Rightarrow> string" where
+  "hexlit 0 0 = ''0x''" |
+  "hexlit len v =
+    (let c = v mod 16 in
+    hexlit (len-1) (v div 16) @ [char_of (if c < 10 then 48 + c else 97 + (c - 10))])"
+
+fun hexliti :: "nat \<Rightarrow> int \<Rightarrow> string" where
+  "hexliti len v = hexlit len (if v < 0 then nat (-v) else nat v)"
+
+instantiation nat :: "show"
+begin
+fun show_nat :: "nat \<Rightarrow> string" where
+  "show_nat n = hexlit 4 n"
+instance proof qed
+end
+
+instantiation int :: "show"
+begin
+fun show_int :: "int \<Rightarrow> string" where
+  "show_int n = hexliti 1 n"
+instance proof qed
+end
+
+instantiation bool :: "show"
+begin
+fun show_bool :: "bool \<Rightarrow> string" where
+  "show_bool True = ''True''" |
+  "show_bool False = ''False''"
+instance proof qed
+end
+
+instantiation instr :: "show"
+begin
+fun show_instr :: "instr \<Rightarrow> string" where
+  "show_instr (JMPZ a) = ''JMPZ '' @ (show a)" |
+  "show_instr ADD = ''ADD''" |
+  "show_instr NOT = ''NOT''" |
+  "show_instr AND = ''AND''" |
+  "show_instr instr.LT = ''LT''" |
+  "show_instr instr.LE = ''LE''" |
+  "show_instr instr.EQ = ''EQ''" |
+  "show_instr (PUSH imm) = ''PUSH '' @ (show imm)" |
+  "show_instr POP = ''POP''" |
+  "show_instr (LID r) = ''LID '' @ (show r)"|
+  "show_instr STORE = ''STORE''" |
+  "show_instr (STOREI r imm) = ''STOREI '' @ (show r) @ '' '' @ (show imm)"|
+  "show_instr COPY = ''COPY''" |
+  "show_instr CALL = ''CALL''" |
+  "show_instr RETURN = ''RETURN''" |
+  "show_instr HALT = ''HALT''" |
+  "show_instr (STOREC n i) = ''STOREC '' @ (show n) @ '' '' @ (show i)" |
+  "show_instr (SETF b) = ''SETF '' @ (show b)"
+instance ..
+end
+
+instantiation prod :: ("show", "show") "show"
+begin
+fun show_prod :: "('a * 'b) \<Rightarrow> string" where
+  "show_prod (a, b) = CHR ''('' # show a @ '', '' @ show b @ '')''"
+instance ..
+end
+
+instantiation list :: ("show") "show"
+begin
+fun show_list_rest :: "'a list \<Rightarrow> string" where
+  "show_list_rest [] = '']''" |
+  "show_list_rest (x # xs) = show x @ '', '' @ show_list_rest xs"
+
+fun show_list :: "'a list \<Rightarrow> string" where
+  "show_list [] = ''[]''" |
+  "show_list xs = show_list_rest xs"
+instance ..
+end
+
+instantiation option :: ("show") "show"
+begin
+fun show_option :: "'a option \<Rightarrow> string" where
+  "show_option None = ''None''" |
+  "show_option (Some x) = ''Some '' @ show x"
+instance ..
+end
+
+abbreviation init where "init \<equiv> (0, [], [], False, [])"
+
+instantiation concrete_program :: "show"
+begin
+fun show_concrete_program :: "concrete_program \<Rightarrow> string" where
+  "show_concrete_program p =
+    (let space = prog_domain p in
+    concat (map (\<lambda>pc. (show pc) @ '' '' @ (show (the (fetch_op p pc))) @ [char_of (10::nat)]) (sorted_list_of_set space)))"
+instance proof qed
+end
+
+definition "asm_width \<equiv> 20"
+datatype 'a dispctx = DisplayCtx concrete_program "'a state_map"
+
+definition "emoji \<equiv> map char_of ([240,159,164,183] :: nat list)"
+
+fun intercalate:: "'a list \<Rightarrow> 'a list list \<Rightarrow> 'a list" where
+  "intercalate _ [] = []" |
+  "intercalate _ [x] = x" |
+  "intercalate sep (x # xs) = x @ sep @ intercalate sep xs"
+
+fun format_ctx_line :: "nat \<Rightarrow> addr \<Rightarrow> program \<Rightarrow> 'a::show \<Rightarrow> string" where
+  "format_ctx_line len pc prog v =
+      (let asm = (show pc) @ '' '' @ (case prog pc of Some op \<Rightarrow> show op | None \<Rightarrow> ''--'');
+           padding = replicate ((asm_width - 1) - length asm + 1) CHR '' '';
+           states = show v in
+      asm @ padding @ states @ ''\<newline>'')"
+
+instantiation dispctx :: ("{show, bot}") "show"
+begin
+fun show_dispctx :: "'a dispctx \<Rightarrow> string" where
+  "show_dispctx (DisplayCtx p st) =
+    concat (map (\<lambda>pc. format_ctx_line asm_width pc (fetch_op p) (lookup st pc)) (sorted_list_of_set (prog_domain p)))"
+instance proof qed
+end
+
+end
